Composition.thy
@@ -1,0 +1,95 @@
+theory Composition
+  imports TM Complexity
+begin
+
+locale TM_switch = TM_abbrevs + M1: TM M1 for M1 :: "('q1, 's, 'l1) TM" +
+  fixes f :: "'l1 \<Rightarrow> ('q2, 's, 'l2) TM"
+  assumes f_tape_count[simp]: "\<And>l. l \<in> M1.labels \<Longrightarrow> TM.k (f l) = M1.k"
+    and symbols_eq[simp]: "\<And>l. l \<in> M1.labels \<Longrightarrow> TM.\<Sigma> (f l) = M1.\<Sigma>"
+begin
+
+lemma tape_symbols_eq[simp]: "\<And>l. l \<in> M1.labels \<Longrightarrow> TM.\<Sigma>\<^sub>t\<^sub>p (f l) = M1.\<Sigma>\<^sub>t\<^sub>p" by simp
+
+lemmas f_simps = f_tape_count symbols_eq tape_symbols_eq
+
+
+abbreviation (input) "switch_TM_states \<equiv> Inl ` M1.Q \<union> Inr ` {(l,q). l \<in> M1.labels \<and> q \<in> TM.Q (f l)}"
+abbreviation (input) "switch_TM_next_state q hds \<equiv>
+  case q of Inl q1 \<Rightarrow>
+    let q1' = M1.\<delta>\<^sub>q q1 hds in
+    if q1' \<in> M1.F
+    then let l = M1.label q1' in Inr (l, TM.q\<^sub>0 (f l))
+    else Inl q1'
+  | Inr (l, q2) \<Rightarrow> Inr (l, TM.\<delta>\<^sub>q (f l) q2 hds)"
+abbreviation (input) "switch_TM_next_write q hds i \<equiv>
+  case q of Inl q1 \<Rightarrow> M1.\<delta>\<^sub>w q1 hds i | Inr (l, q2) \<Rightarrow> TM.\<delta>\<^sub>w (f l) q2 hds i"
+abbreviation (input) "switch_TM_next_move q hds i \<equiv>
+  case q of Inl q1 \<Rightarrow> M1.\<delta>\<^sub>m q1 hds i | Inr (l, q2) \<Rightarrow> TM.\<delta>\<^sub>m (f l) q2 hds i"
+
+definition switch_TM_rec :: "('q1 + ('l1 \<times> 'q2), 's, 'l2) TM_record"
+  where "switch_TM_rec \<equiv> \<lparr>
+    TM_record.tape_count = M1.k,
+    symbols = M1.\<Sigma>,
+    states = switch_TM_states,
+    initial_state = Inl M1.q\<^sub>0,
+    final_states = Inr ` {(l,q). l \<in> M1.labels \<and> q \<in> TM.F (f l)},
+    label = \<lambda>q. case q of Inr (l, q2) \<Rightarrow> TM.label (f l) q2,
+    next_state = switch_TM_next_state,
+    next_write = switch_TM_next_write,
+    next_move  = switch_TM_next_move
+  \<rparr>"
+
+lemma valid_switch_TM: "valid_TM switch_TM_rec" unfolding switch_TM_rec_def
+proof (intro valid_TM_I)
+  let ?Q = switch_TM_states and ?\<delta>\<^sub>q = switch_TM_next_state and ?\<delta>\<^sub>w = switch_TM_next_write
+
+  have h1: "{(l, q). l \<in> M1.labels \<and> q \<in> TM.Q (f l)} = (\<Union>l\<in>M1.labels. Pair l ` TM.Q (f l))" by blast
+  have "finite (\<Union>l\<in>M1.labels. Pair l ` TM.Q (f l))" by blast
+  then show "finite ?Q" unfolding h1 by blast
+
+  fix q hds
+  assume q: "q \<in> ?Q"
+  assume hds: "length hds = M1.k" "set hds \<subseteq> M1.\<Sigma>\<^sub>t\<^sub>p"
+
+  show "?\<delta>\<^sub>q q hds \<in> ?Q" using q
+  proof (induction q)
+    case (Inl q1)
+    then have q1: "q1 \<in> M1.Q" by blast
+    with hds show ?case unfolding sum.case Let_def by (induction rule: ifI) blast+
+  next
+    case (Inr q2)
+    then have "q2 \<in> {(l, q). l \<in> M1.labels \<and> q \<in> TM.Q (f l)}" by blast
+    then show ?case unfolding sum.case
+    proof (induction q2)
+      case (Pair l q2')
+      then have l: "l \<in> M1.labels" and q2': "q2' \<in> TM.Q (f l)" by blast+
+      with hds have "TM.\<delta>\<^sub>q (f l) q2' hds \<in> TM.Q (f l)" by force
+      with l show ?case unfolding prod.case by blast
+    qed
+  qed
+
+  fix i
+  assume i: "i < M1.k"
+
+  show "?\<delta>\<^sub>w q hds i \<in> M1.\<Sigma>\<^sub>t\<^sub>p" using q
+  proof (induction q)
+    case (Inl q1)
+    then have q1: "q1 \<in> M1.Q" by blast
+    with hds i show ?case unfolding sum.case by blast
+  next
+    case (Inr q2)
+    then have "q2 \<in> {(l, q). l \<in> M1.labels \<and> q \<in> TM.Q (f l)}" by blast
+    then show ?case unfolding sum.case
+    proof (induction q2)
+      case (Pair l q2')
+      then have l: "l \<in> M1.labels" and q2': "q2' \<in> TM.Q (f l)" by blast+
+      with hds i have "TM.\<delta>\<^sub>w (f l) q2' hds i \<in> TM.\<Sigma>\<^sub>t\<^sub>p (f l)"
+        by (intro TM.next_write_valid) (unfold f_simps[OF l])
+      then show ?case using l by simp
+    qed
+  qed
+qed (use M1.symbol_axioms(2) in blast)+
+
+end \<comment> \<open>\<^locale>\<open>TM_switch\<close>\<close>
+
+end
